Stuck at functionality of evaluation because we cannot get true equality due to propoof irrelevance in prop, going to try to remove rule annotations

theories/PtsSignature.v
@@ -6,8 +6,8 @@ Record PtsSig : Type :=
   mkPtsSig {
       St :> Set;
       Ax : St -> St -> Prop;
-      Ru : St -> St -> St -> Set;
-      Ru_nat : St -> Set;
+      Ru : St -> St -> St -> Prop;
+      Ru_nat : St -> Prop;
     }.
 
 Record PredicativeSig (P : PtsSig) : Type :=
@@ -77,10 +77,10 @@ Section SignatureExtension.
   | ax_ext : forall {n : nat}, eAx (st_ext n) (st_ext (S n))
   | ax_cross : forall {s : St P}, eAx (st_P s) (st_ext 0).
 
-  Inductive eRu : eSt -> eSt -> eSt -> Set :=
+  Inductive eRu : eSt -> eSt -> eSt -> Prop :=
   | ru_P : forall {s1 s2 s3 : St P}, Ru P s1 s2 s3 -> eRu (st_P s1) (st_P s2) (st_P s3).
 
-  Inductive eRu_nat : eSt -> Set :=
+  Inductive eRu_nat : eSt -> Prop :=
   | runat_P : forall {s : St P}, Ru_nat P s -> eRu_nat (st_P s).
 
   Definition eP : PtsSig := mkPtsSig eSt eAx eRu eRu_nat.
